%----------------------------------------------------------------------------------------
%	PROBLEM 1
%----------------------------------------------------------------------------------------

\section{Problem I}
Sort the following functions from asymptotically smallest to asymptotically largest.

\begin{center}
	$ 2^{log_{10}{n}} \quad log_{lg{n}}{n} \quad  lg(nlog{n})  \quad  n \quad (\sqrt{2})^{lg{n}} \quad (lglgn)^{lglgn} $
\end{center}

\textbf{Solution:} \\

We could find that
$$\lim_{n\to\infty} \frac{\sqrt{2}^{lgn}}{n} = \lim_{n\to\infty} \frac{n^{0.5}}{n} = \lim_{n\to\infty} \frac{1}{n^{0.5}} = 0$$
So 
$$\sqrt{2}^{lgn} = o(n)$$

Similarly we have
$$\lim_{n\to\infty} \frac{2^{log_{10}n}}{\sqrt{2}^{lgn}} = \lim_{n\to\infty} \frac{n^{log_{10}2}}{n^{0.5}} = \lim_{n\to\infty} \frac{1}{n^{0.5 - log_{10}2}}$$
since $0.5 - log_{10}2 > 0$
$$ \lim_{n\to\infty} \frac{1}{n^{0.5 - log_{10}2}} = 0 $$
So 
$$ 2^{log_{10}n} = o(\sqrt{2}^{lgn})$$

To compare $2^{log_{10}n}$ and $(lglgn)^{lglgn}$,\\
We apply $log()$ on both side\\
LHS:
$$lg(2^{log_{10}n}) = lg_{10}2lgn$$
RHS:
$$lg((lglgn)^{lglgn}) = lglgn\cdot lglglgn < (lglgn)^2$$
Then we have:
$$ \lim_{n\to\infty} \frac{(lglgn)^2}{lg_{10}2lgn} = \lim_{n\to\infty} \frac{2lglgn}{log_{10}2ln2lgn}  = \lim_{n\to\infty} \frac{2}{log_{10}2ln^22lgn} = 0$$
Then we have
$$ (lglgn)^2 = o(2^{log_{10}n}) $$
And $lglgn\cdot lglglgn < (lglgn)^2$, so
$$ (lglgn)^{lglgn} = o(2^{log_{10}n}) $$

To compare $(lglgn)^{lglgn}$ and $lg(nlog{n})$,\\
We apply $log()$ on both side\\
LHS:
$$log(lg(nlog{n})) = lg(lgn + lglgn) < lg(2lgn)$$
RHS:
$$log((lglgn)^{lglgn}) = lglgn\cdot lglglgn$$
Then we have:
$$\lim_{n\to\infty} \frac{lg(2lgn)}{lglgn\cdot lglglgn} = \lim_{n\to\infty} \frac{1 + lglgn}{lglgn\cdot lglglgn}  = \lim_{n\to\infty} \frac{1}{lglgn\cdot lglglgn} + \frac{1}{lglglgn} = 0$$
Then we have
$$ lg(2lgn) = o(lglgn\cdot lglglgn) $$
And $lg(lgn + lglgn) < lg(2lgn)$, so
$$ lg(nlog{n}) = o((lglgn)^{lglgn}) $$

To compare $log_{lg{n}}{n}$ and $lg(nlog{n})$,\\
LHS:
$$log_{lg{n}}{n} = \frac{lgn}{lglgn}$$
RHS:
$$lg(nlog{n}) = lgn + lglgn > lgn$$
Then we have:
$$\lim_{n\to\infty} \frac{\frac{lgn}{lglgn}}{lgn} = 0$$
So, 
$$log_{lg{n}}{n} = \frac{lgn}{lglgn} = o(lgn)$$
Since,
$$lgn + lglgn > lgn$$
Therefore, 
$$log_{lg{n}}{n} = o(lgn + lglgn) = o(lg(nlog{n}))$$

In conlusion, 
$$n >> (\sqrt{2})^{lg{n}} >> 2^{log_{10}{n}} >> (lglgn)^{lglgn} >> lg(nlog{n}) >> log_{lg{n}}{n}$$
